Attempts at destruct_fs_beh lemma.

rupicola/io/IO.fst
@@ -14,6 +14,8 @@ type io (a:Type u#a) : Type u#a =
 let io_return (#a:Type) (x:a) : io a =
   Return x
 
+let extract_v_from_io_return (#a:Type) (m:(io a){exists x. m == io_return x}) : (x:a{io_return x == m}) = admit ()
+
 let rec io_bind
   (#a:Type u#a)
   (#b:Type u#b)
@@ -82,3 +84,386 @@ let lem_theta_write arg res h =
 
 let lem_theta_close arg res h =
   assert (thetaP (close arg) h [EvClose arg res] res) by (compute ())
+
+(*let rec destruct_fs_beh_m #t1 #t2 (m:io t1) (w:t1 -> hist t2) (h:history) (lt:local_trace h) (fs_r:t2) :
+  Lemma (requires forall p. hist_bind (theta m) w h p ==> p lt fs_r) 
+        (ensures exists (lt1:local_trace h) (fs_m:t1). forall p. theta m h p ==> p lt1 fs_m) =
+  match m with
+  | Return x -> ()
+  | Call o args k -> begin
+    match lt with
+    | [] -> admit ()
+    | ev::tl -> begin
+      let r : io_res o (magic ()) = magic () in
+      
+       destruct_fs_beh_m (k r) w (h++[ev]) tl fs_r;
+       admit ()
+      
+   end
+  end
+
+let destruct_fs_beh_m #t1 #t2 (m:io t1) (k:t1 -> io t2) (h:history) (lt:local_trace h) (fs_r:t2) :
+  Lemma (requires thetaP (io_bind m k) h lt fs_r)
+        (ensures exists (lt1:local_trace h) (fs_m:t1). thetaP m h lt1 fs_m) =
+  wp2p_theta_bind m k;
+  assert (wp2p (hist_bind (theta m) (fun x -> theta (k x))) h lt fs_r);
+  assert (forall p. hist_bind (theta m) (fun x -> theta (k x)) h p ==> p lt fs_r);
+  assert (forall p. (theta m) h (fun lt r -> theta (k r) (fun lt' r' -> p (lt@lt') r')) ==> p lt fs_r);
+  assert (theta m h (fun lt r -> True));
+   introduce exists (lt1:local_trace h) (fs_m:t1). forall p. theta m h p ==> p lt1 fs_m with _ _
+  //assert (forall p. (theta (io_bind m k)) h p ==> p lt fs_m);
+
+#push-options "--split_queries always"
+let rec destruct_fs_beh' #t1 #t2 (m:io t1) (k:t1 -> io t2) (h:history) (lt:local_trace h) (fs_r:t2) :
+  //Pure ((lt1:local_trace h & local_trace (h++lt1)) * t1)
+  Lemma
+    (requires thetaP (io_bind m k) h lt fs_r)
+    (*(ensures fun ((| lt1, lt2 |), fs_m) ->
+      lt == (lt1@lt2) /\ 
+      thetaP m h lt1 fs_m /\ 
+      thetaP (k fs_m) (h++lt1) lt2 fs_r)*)
+    (ensures exists (lt1:local_trace h) (lt2:local_trace (h++lt1)) (fs_m:t1). 
+      lt == (lt1@lt2) /\ 
+      thetaP m h lt1 fs_m /\ 
+      thetaP (k fs_m) (h++lt1) lt2 fs_r)
+    (decreases m) =
+  match m with
+  | Return x -> begin
+    admit ()
+    end
+  | Call o args fnc -> begin
+    match lt with
+    | [] -> admit ()
+    | ev::tl -> begin
+      match o with
+      | ORead -> begin
+        assert (thetaP (io_bind m k) h lt fs_r == wp2p (theta (io_bind m k)) h lt fs_r);
+        assert (wp2p (theta (io_bind m k)) h lt fs_r <==> forall p. (theta (io_bind m k)) h p ==> p lt fs_r);
+        assert (forall p. (theta (Call ORead args (fun i -> io_bind #t1 #t2 (fnc i) k)) h p ==> p (ev::tl) fs_r));
+        assert (forall p. hist_bind (op_wp ORead args) (fun r -> theta (io_bind #t1 #t2 (fnc r) k)) h p ==> p (ev::tl) fs_r);
+        let p : hist_post h t2 = fun lt res -> exists res' lt'. lt == ((EvRead args res')::lt') in
+        assert (hist_bind (op_wp ORead args) (fun r -> theta (io_bind #t1 #t2 (fnc r) k)) h p ==> p (ev::tl) fs_r);
+        assert (hist_bind (op_wp ORead args) (fun r -> theta (io_bind #t1 #t2 (fnc r) k)) h p == (op_wp ORead args) h (hist_post_bind' (fun r -> theta (io_bind #t1 #t2 (fnc r) k)) p)) by (FStar.Tactics.compute ());
+        assert ((op_wp ORead args) h (hist_post_bind' (fun r -> theta (io_bind #t1 #t2 (fnc r) k)) p) == (to_hist (fun h -> io_pre h ORead args) (fun h res lt -> io_post h ORead args res /\ lt == [op_to_ev ORead args res])) h (hist_post_bind' (fun r -> theta (io_bind #t1 #t2 (fnc r) k)) p)) by (FStar.Tactics.compute ());
+        //assert ((to_hist (fun h -> io_pre h ORead args) (fun h res lt -> io_post h ORead args res /\ lt == [op_to_ev ORead args res])) h (hist_post_bind' (fun r -> theta (io_bind #t1 #t2 (fnc r) k)) p) == 
+        assert (io_pre h ORead args);
+        //***assert (forall lt r. io_post h ORead args r /\ lt == [op_to_ev ORead args r] ==> (hist_post_bind' (fun r -> theta (io_bind #t1 #t2 (fnc r) k)) p) lt r);
+        assume (forall lt r. io_post h ORead args r /\ lt == [op_to_ev ORead args r] ==> theta (io_bind #t1 #t2 (fnc r) k) (h++lt) (fun lt' r -> p (lt @ lt') r));
+        assert (p (ev::tl) fs_r);
+        //assert (lt == ([EvRead args fs_r]@lt2)); 
+      //thetaP m h lt1 fs_m /\ 
+      //thetaP (k fs_m) (h++lt1) lt2 fs_r
+        admit ()
+        end
+      | OWrite -> admit ()
+      | OOpen -> admit ()
+      | OClose -> admit ()
+      end
+    end
+#pop-options*)
+
+(*let theta_lemma #t1 #t2 (args:io_args ORead) (cont_m:io_res ORead args -> io t1) (k:t1 -> io t2) (h:history) (p:hist_post h t2):
+  Lemma 
+    (requires theta (io_bind (Call ORead args cont_m) k) h p) 
+    (ensures forall (lt':local_trace h) (r':io_res ORead args). io_pre h ORead args /\ (io_post h ORead args r' /\ lt' == [op_to_ev ORead args r']) ==> theta (io_bind #t1 #t2 (cont_m r') k) (h++lt') (fun lt'' r'' -> p (lt' @ lt'') r'')) = admit ()*)// this is by definition
+
+let test #t1 #t2 (args:io_args ORead) (res:io_res ORead args) (cont_m:io_res ORead args -> io t1) (k:t1 -> io t2) (h:history) (tl:local_trace (h++[EvRead args res])) (fs_r:t2) (p:hist_post h t2) :
+  Lemma (requires (theta (io_bind (Call ORead args cont_m) k) h p ==> p ([EvRead args res]@tl) fs_r) /\ theta (io_bind (Call ORead args cont_m) k) h p)
+        (ensures (theta (io_bind (cont_m res) k) (h++[EvRead args res]) (fun (lt'':local_trace (h++[EvRead args res])) (r'':t2) -> p ([EvRead args res] @ lt'') r'') ==> (fun lt'' r'' -> p ([EvRead args res] @ lt'') r'') tl fs_r)) = ()
+
+let test2 #t1 #t2 (o:io_ops) (args:io_args o) (res:io_res o args) (cont_m:io_res o args -> io t1) (k:t1 -> io t2) (h:history) (tl:local_trace (h++[op_to_ev o args res])) (fs_r:t2) (p:hist_post h t2) :
+  Lemma (requires (theta (io_bind (Call o args cont_m) k) h p) /\ p ([op_to_ev o args res]@tl) fs_r)
+        (ensures (theta (io_bind (cont_m res) k) (h++[op_to_ev o args res]) (fun (lt'':local_trace (h++[op_to_ev o args res])) (r'':t2) -> p ([op_to_ev o args res] @ lt'') r'')) /\ (fun (lt'':local_trace (h++[op_to_ev o args res])) (r'':t2) -> p ([op_to_ev o args res] @ lt'') r'') tl fs_r) =
+  assert (theta (io_bind (Call o args cont_m) k) h p);
+  assert (theta (Call o args (fun (i:io_res o args) -> io_bind #t1 #t2 (cont_m i) k)) h p);
+  assert (hist_bind (op_wp o args) (fun r -> theta ((fun i -> io_bind #t1 #t2 (cont_m i) k) r)) h p);
+  assert (hist_bind (op_wp o args) (fun r -> theta (io_bind #t1 #t2 (cont_m r) k)) h p);
+  assert ((op_wp o args) h (hist_post_bind' (fun r -> theta (io_bind #t1 #t2 (cont_m r) k)) p));
+  assert ((op_wp o args) h (fun lt_ r_ -> theta (io_bind #t1 #t2 (cont_m r_) k) (h++lt_) (hist_post_shift h p lt_)));
+  assert ((op_wp o args) h (fun lt_ r_ -> theta (io_bind #t1 #t2 (cont_m r_) k) (h++lt_) (fun lt_' r_' -> p (lt_ @ lt_') r_')));
+  assert ((op_wp o args) == (to_hist (fun h -> io_pre h o args) (fun h res' lt' -> io_post h o args res' /\ lt' == [op_to_ev o args res']))) by (FStar.Tactics.compute ());
+  assert ((to_hist (fun h -> io_pre h o args) (fun h res' lt' -> io_post h o args res' /\ lt' == [op_to_ev o args res'])) h (hist_post_bind' (fun r -> theta (io_bind #t1 #t2 (cont_m r) k)) p) <==> (io_pre h o args /\ (forall (lt':local_trace h) (r':io_res o args). (io_post h o args r' /\ lt' == [op_to_ev o args r']) ==> theta (io_bind #t1 #t2 (cont_m r') k) (h++lt') (fun lt'' r'' -> p (lt' @ lt'') r''))));
+  assume ((to_hist (fun h -> io_pre h o args) (fun h res' lt' -> io_post h o args res' /\ lt' == [op_to_ev o args res'])) h (fun lt_ r_ -> theta (io_bind #t1 #t2 (cont_m r_) k) (h++lt_) (fun lt_' r_' -> p (lt_ @ lt_') r_')));
+  assert (io_pre h o args /\ (forall (lt':local_trace h) (r':io_res o args). (io_post h o args r' /\ lt' == [op_to_ev o args r']) ==> theta (io_bind #t1 #t2 (cont_m r') k) (h++lt') (fun lt'' r'' -> p (lt' @ lt'') r'')));
+  assert (io_pre h o args);
+  eliminate forall (lt':local_trace h) (r':io_res o args). (io_post h o args r' /\ lt' == [op_to_ev o args r']) ==> theta (io_bind #t1 #t2 (cont_m r') k) (h++lt') (fun lt'' r'' -> p (lt' @ lt'') r'') with [op_to_ev o args res] res;
+  assert ((io_post h o args res /\ [op_to_ev o args res] == [op_to_ev o args res]) ==> theta (io_bind #t1 #t2 (cont_m res) k) (h++[op_to_ev o args res]) (fun lt'' r'' -> p ([op_to_ev o args res] @ lt'') r''));
+  ()
+
+let test2' #t1 #t2 (o:io_ops) (args:io_args o) (cont_m:io_res o args -> io t1) (k:t1 -> io t2) (h:history) (ev:event_h h) (tl:local_trace (h++[ev])) (lt:local_trace h{lt == (ev::tl)}) (fs_r:t2) (p:hist_post h t2) :
+  Lemma (requires (theta (io_bind (Call o args cont_m) k) h p) /\ p (ev::tl) fs_r)
+        (ensures forall (res:io_res o args). (theta (io_bind (cont_m res) k) (h++[ev]) (fun (lt'':local_trace (h++[ev])) (r'':t2) -> p ([ev] @ lt'') r'')) /\ (fun (lt'':local_trace (h++[ev])) (r'':t2) -> p ([ev] @ lt'') r'') tl fs_r) =
+  assert (theta (io_bind (Call o args cont_m) k) h p);
+  assert (theta (Call o args (fun (i:io_res o args) -> io_bind #t1 #t2 (cont_m i) k)) h p);
+  assert (hist_bind (op_wp o args) (fun r -> theta ((fun i -> io_bind #t1 #t2 (cont_m i) k) r)) h p);
+  assert (hist_bind (op_wp o args) (fun r -> theta (io_bind #t1 #t2 (cont_m r) k)) h p);
+  assert ((op_wp o args) h (hist_post_bind' (fun r -> theta (io_bind #t1 #t2 (cont_m r) k)) p));
+  assert ((op_wp o args) h (fun lt_ r_ -> theta (io_bind #t1 #t2 (cont_m r_) k) (h++lt_) (hist_post_shift h p lt_)));
+  assert ((op_wp o args) h (fun lt_ r_ -> theta (io_bind #t1 #t2 (cont_m r_) k) (h++lt_) (fun lt_' r_' -> p (lt_ @ lt_') r_')));
+  assert ((op_wp o args) == (to_hist (fun h -> io_pre h o args) (fun h res' lt' -> io_post h o args res' /\ lt' == [op_to_ev o args res']))) by (FStar.Tactics.compute ());
+  assert ((to_hist (fun h -> io_pre h o args) (fun h res' lt' -> io_post h o args res' /\ lt' == [op_to_ev o args res'])) h (hist_post_bind' (fun r -> theta (io_bind #t1 #t2 (cont_m r) k)) p) <==> (io_pre h o args /\ (forall (lt':local_trace h) (r':io_res o args). (io_post h o args r' /\ lt' == [op_to_ev o args r']) ==> theta (io_bind #t1 #t2 (cont_m r') k) (h++lt') (fun lt'' r'' -> p (lt' @ lt'') r''))));
+  assume ((to_hist (fun h -> io_pre h o args) (fun h res' lt' -> io_post h o args res' /\ lt' == [op_to_ev o args res'])) h (fun lt_ r_ -> theta (io_bind #t1 #t2 (cont_m r_) k) (h++lt_) (fun lt_' r_' -> p (lt_ @ lt_') r_')));
+  assert (io_pre h o args /\ (forall (lt':local_trace h) (r':io_res o args). (io_post h o args r' /\ lt' == [op_to_ev o args r']) ==> theta (io_bind #t1 #t2 (cont_m r') k) (h++lt') (fun lt'' r'' -> p (lt' @ lt'') r'')));
+  assert (io_pre h o args);
+  introduce forall (res:io_res o args). (theta (io_bind (cont_m res) k) (h++[ev]) (fun (lt'':local_trace (h++[ev])) (r'':t2) -> p ([ev] @ lt'') r'')) /\ (fun (lt'':local_trace (h++[ev])) (r'':t2) -> p ([ev] @ lt'') r'') tl fs_r with begin
+      eliminate forall (lt':local_trace h) (r':io_res o args). (io_post h o args r' /\ lt' == [op_to_ev o args r']) ==> theta (io_bind #t1 #t2 (cont_m r') k) (h++lt') (fun lt'' r'' -> p (lt' @ lt'') r'') with [ev] res;
+      //assert ((io_post h o args res /\ [ev] == [op_to_ev o args res]) <==> theta (io_bind #t1 #t2 (cont_m res) k) (h++[ev]) (fun lt'' r'' -> p ([ev] @ lt'') r''));
+      assume ([ev] == [op_to_ev o args res]);
+      ()
+    end
+    
+let testing_something #t1 #t2 (m:io t1) (k:t1 -> io t2) (h:history) (lt:local_trace h) (fs_r:t2) (p:hist_post h t2) :
+  Lemma (ensures (theta (io_bind m k) h p ==> p lt fs_r) <==> (theta (io_bind m k) h (hist_post_bind (fun (lt':local_trace h) (r:t1) -> theta (k r) (h++lt') (fun (lt'':local_trace (h++lt')) (r':t2) -> p (lt' @ lt'') r')) (fun (lt':local_trace h) (r:t1) -> (fun (lt'':local_trace (h++lt')) (r':t2) -> p (lt' @ lt'') r'))) ==> (hist_post_bind (fun (lt':local_trace h) (r:t1) -> theta (k r) (h++lt') (fun (lt'':local_trace (h++lt')) (r':t2) -> p (lt' @ lt'') r')) (fun (lt':local_trace h) (r:t1) -> (fun (lt'':local_trace (h++lt')) (r':t2) -> p (lt' @ lt'') r'))) lt fs_r)) = admit ()
+
+let more_testing #t1 #t2 (m:io t1) (k:t1 -> io t2) (h:history) (p:hist_post h t1) (fs_r:t2) :
+  Lemma (requires theta m h p) // p lta a /\ lta@ltb == lt /\ k_ lta a ltb b
+        (ensures theta (io_bind m k) h (hist_post_bind p (fun (lt:local_trace h) (r:t1) -> (fun (lt':local_trace (h++lt)) (r':t2) -> r' == fs_r)))) = admit ()
+
+let more_testing' #t1 #t2 (m:io t1) (k:t1 -> io t2) (h:history) (lt:local_trace h) (fs_r:t2) :
+  Lemma (requires forall (p:hist_post h t2). theta m h (fun (lt':local_trace h) (r:t1) -> theta (k r) (h++lt') (fun (lt'':local_trace (h++lt')) (r':t2) -> p (lt' @ lt'') r')) ==> p lt fs_r)
+        (ensures forall (p:hist_post h t2). theta (io_bind m k) h (hist_post_bind (fun (lt':local_trace h) (r:t1) -> theta (k r) (h++lt') (fun (lt'':local_trace (h++lt')) (r':t2) -> p (lt' @ lt'') r')) (fun (lt:local_trace h) (r:t1) -> (fun (lt':local_trace (h++lt)) (r':t2) -> r' == fs_r))) ==> (hist_post_bind (fun (lt':local_trace h) (r:t1) -> theta (k r) (h++lt') (fun (lt'':local_trace (h++lt')) (r':t2) -> p (lt' @ lt'') r')) (fun (lt:local_trace h) (r:t1) -> (fun (lt':local_trace (h++lt)) (r':t2) -> r' == fs_r))) lt fs_r) = admit ()
+
+let final_test #t1 #t2 (m:io t1) (k:t1 -> io t2) (h:history) (lt:local_trace h) (fs_r:t2) :
+  Lemma (requires forall (p:hist_post h t2). theta (io_bind m k) h p ==> p lt fs_r)
+        (ensures forall (p':hist_post h t1). theta m h p' ==> (exists (fs_r_m:t1) (lt1:local_trace h) (lt2:local_trace (h++lt1)). p' lt1 fs_r_m /\ (lt1@lt2 == lt))) =
+  introduce forall p'. theta m h p' ==> (exists (fs_r_m:t1) (lt1:local_trace h) (lt2:local_trace (h++lt1)). p' lt1 fs_r_m /\ (lt1@lt2 == lt)) with begin
+    introduce _ ==> _ with _. begin
+      more_testing m k h p' fs_r;
+      assert ((hist_post_bind p' (fun (lt:local_trace h) (r:t1) -> (fun (lt':local_trace (h++lt)) (r':t2) -> r' == fs_r))) lt fs_r);
+      assert ((fun (lt:local_trace h) (r:t2) -> exists (fs_r_m:t1) (lt1:local_trace h) (lt2:local_trace (h++lt1)). p' lt1 fs_r_m /\ lt1@lt2 == lt /\ r == fs_r) lt fs_r);
+      ()
+    end
+  end
+
+let uniqueness_of_result #t1 (m:io t1) (h:history) (p:hist_post h t1) :
+  Lemma (forall (lt lt':local_trace h) (r r':t1). (p lt r /\ p lt' r') ==> ((lt == lt') /\ (r' == r))) = admit ()
+
+let most_testing #t1 (m:io t1) (h:history) (lt1':local_trace h) (fs_r_m':t1) :
+  Lemma (requires forall (p':hist_post h t1). theta m h p' ==> (exists (fs_r_m:t1) (lt1:local_trace h) (lt2:local_trace (h++lt1)). p' lt1 fs_r_m))
+        (ensures forall (p':hist_post h t1). theta m h p' ==> p' lt1' fs_r_m') = 
+ introduce forall (p':hist_post h t1). theta m h p' ==> p' lt1' fs_r_m' with begin
+   introduce _ ==> _ with _. begin
+     eliminate forall (p':hist_post h t1). theta m h p' ==> (exists (fs_r_m:t1) (lt1:local_trace h) (lt2:local_trace (h++lt1)). p' lt1 fs_r_m) with p';
+     uniqueness_of_result m h p';
+     admit ()
+   end
+ end
+
+#push-options "--split_queries always"
+let rec test_m #t1 #t2 (m:io t1) (k:t1 -> io t2) (h:history) (lt:local_trace h) (fs_r:t2) (p:hist_post h t2) :
+  Pure (t1 * (lt1:local_trace h & local_trace (h++lt1))) 
+    (requires theta (io_bind m k) h p /\ p lt fs_r)
+    (ensures fun (fs_r_m, (| lt1, lt2 |)) ->
+      lt == (lt1@lt2) /\
+      theta (k fs_r_m) (h++lt1) (fun (lt'':local_trace (h++lt1)) (r'':t2) -> p (lt1@lt'') r'') ==> (fun lt'' r'' -> p (lt1@lt'') r'') lt2 fs_r)
+    (decreases m) =
+    theta_monad_morphism_bind m k;
+    assert (theta (io_bind m k) `hist_equiv` hist_bind (theta m) (fun x -> theta (k x)));
+    assert ((theta (io_bind m k)) h p <==> (hist_bind (theta m) (fun x -> theta (k x))) h p);
+    assert (theta (io_bind m k) h p);
+    assert ((hist_bind (theta m) (fun x -> theta (k x))) h p);
+    assert ((theta m) h (hist_post_bind' (fun x -> theta (k x)) p));
+    assert ((theta m) h (fun lt' r -> theta (k r) (h++lt') (hist_post_shift h p lt')));
+    assert ((theta m) h (fun (lt':local_trace h) (r:t1) -> theta (k r) (h++lt') (fun (lt'':local_trace (h++lt')) (r':t2) -> p (lt' @ lt'') r')));
+    assert (p lt fs_r);
+    let _ : hist_post h t2 = p in
+    let m_ : hist_post h t1 = (fun (lt':local_trace h) (r:t1) -> theta (k r) (h++lt') (fun (lt'':local_trace (h++lt')) (r':t2) -> p (lt' @ lt'') r')) in
+    let k_ : (lt:local_trace h -> t1 -> hist_post (h++lt) t2) = fun (lt':local_trace h) (r:t1) -> (fun (lt'':local_trace (h++lt')) (r':t2) -> p (lt' @ lt'') r') in
+    let p1 : hist_post h t2 = hist_post_bind m_ k_ in
+    assert (hist_post_bind m_ k_ == (fun (lt:local_trace h) (b:t2) -> exists (a:t1) (lta:local_trace h) (ltb:local_trace (h++lta)). m_ lta a /\ lta@ltb == lt /\ k_ lta a ltb b)) by (FStar.Tactics.compute ());
+    introduce forall lt r. p1 lt r ==> p lt r with begin
+      introduce _ ==> _ with _. begin
+        ()
+      end
+    end;
+    assert (p1 `hist_post_ord` p);
+    assert (hist_wp_monotonic (theta (io_bind m k)));
+    assert ((theta (io_bind m k)) h p1 ==> (theta (io_bind m k)) h p);
+    //assert ((theta (io_bind m k)) h p1);
+    (*assert (p1 lt fs_r);
+    assert (exists (a:t1) (lta:local_trace h) (ltb:local_trace (h++lta)). m_ lta a /\ lta@ltb == lt /\ k_ lta a ltb fs_r);*)
+    
+    admit ()
+#pop-options
+    (*match m with
+    | Return x -> (x, (| [], lt |))
+    | Call o args cont_m -> begin
+      assert (theta (io_bind m k) h p);
+      match lt with
+      | [] -> admit () // should be false_elim ()
+      | (ev::tl) -> begin
+        assert (theta (io_bind (Call o args cont_m) k) h p /\ p (ev::tl) fs_r);
+        assume (well_formed_local_trace (h++[ev]) tl);
+        test2' o args cont_m k h ev tl (ev::tl) fs_r p;
+        //eliminate forall (res:io_res o args). (theta (io_bind (cont_m res) k) (h++[ev]) (fun (lt'':local_trace (h++[ev])) (r'':t2) -> p ([ev] @ lt'') r'')) /\ (fun (lt'':local_trace (h++[ev])) (r'':t2) -> p ([ev] @ lt'') r'') tl fs_r 
+        //let (fs_r_m', (| lt1', lt2' |)) = test_m (cont_m_ res_) k (h++[op_to_ev o_ args_ res_]) tl fs_r (fun (lt'':local_trace (h++[op_to_ev o_ args_ res_])) (r'':t2) -> p ([op_to_ev o_ args_ res_] @ lt'') r'') in
+        //(fs_r_m', (| ([op_to_ev o_ args_ res_]@lt1'), lt2' |))
+        admit ()
+        end
+      end*)
+
+let destruct_fs_beh_small #t1 #t2 (args:io_args ORead) (res:io_res ORead args) (cont_m:io_res ORead args -> io t1) (k:t1 -> io t2) (h:history) (tl:local_trace (h++[EvRead args res])) (fs_r:t2) :
+  Lemma (requires thetaP (io_bind (Call ORead args cont_m) k) h ([EvRead args res]@tl) fs_r)
+        (ensures thetaP (io_bind (cont_m res) k) (h++[EvRead args res]) tl fs_r) =
+  assert (forall (p:hist_post h t2). theta (io_bind (Call ORead args cont_m) k) h p ==> p ([EvRead args res]@tl) fs_r);
+  assert (forall (p:hist_post h t2). theta (Call ORead args (fun (i:io_res ORead args) -> io_bind #t1 #t2 (cont_m i) k)) h p ==> p ([EvRead args res]@tl) fs_r);
+  assert (forall (p:hist_post h t2). hist_bind (op_wp ORead args) (fun r -> theta ((fun i -> io_bind #t1 #t2 (cont_m i) k) r)) h p ==> p ([EvRead args res]@tl) fs_r);
+  assert (forall (p:hist_post h t2). hist_bind (op_wp ORead args) (fun r -> theta (io_bind #t1 #t2 (cont_m r) k)) h p ==> p ([EvRead args res]@tl) fs_r);
+  assert (forall (p:hist_post h t2). (op_wp ORead args) h (hist_post_bind' (fun r -> theta (io_bind #t1 #t2 (cont_m r) k)) p) ==> p ([EvRead args res]@tl) fs_r);
+  assert (forall (p:hist_post h t2). (to_hist (fun h -> io_pre h ORead args) (fun h res lt -> io_post h ORead args res /\ lt == [op_to_ev ORead args res])) h (hist_post_bind' (fun r -> theta (io_bind #t1 #t2 (cont_m r) k)) p) ==> p ([EvRead args res]@tl) fs_r);
+  assert (forall (p:hist_post h t2). (to_hist (fun h -> io_pre h ORead args) (fun h res lt -> io_post h ORead args res /\ lt == [op_to_ev ORead args res])) h (hist_post_bind' (fun r -> theta (io_bind #t1 #t2 (cont_m r) k)) p) <==> (io_pre h ORead args /\ (forall (lt':local_trace h) (r':io_res ORead args). (io_post h ORead args r' /\ lt' == [op_to_ev ORead args r']) ==> theta (io_bind #t1 #t2 (cont_m r') k) (h++lt') (fun lt'' r'' -> p (lt' @ lt'') r''))));
+  assert (forall (p:hist_post h t2). (io_pre h ORead args /\ (forall (lt':local_trace h) (r':io_res ORead args). (io_post h ORead args r' /\ lt' == [op_to_ev ORead args r']) ==> theta (io_bind #t1 #t2 (cont_m r') k) (h++lt') (fun lt'' r'' -> p (lt' @ lt'') r''))) ==> p ([EvRead args res]@tl) fs_r);
+  introduce forall (p':hist_post (h++[EvRead args res]) t2). theta (io_bind (cont_m res) k) (h++[EvRead args res]) p' ==> p' tl fs_r with begin
+    introduce _ ==> _ with _. begin
+      let p : hist_post h t2 = fun (lt'':local_trace h) (r'':t2) -> exists (tl:local_trace (h++[EvRead args res])). lt'' == [EvRead args res]@tl /\ p' tl r'' in
+      eliminate forall (p:hist_post h t2). (io_pre h ORead args /\ (forall (lt':local_trace h) (r':io_res ORead args). (io_post h ORead args r' /\ lt' == [op_to_ev ORead args r']) ==> theta (io_bind #t1 #t2 (cont_m r') k) (h++lt') (fun lt'' r'' -> p (lt' @ lt'') r''))) ==> p ([EvRead args res]@tl) fs_r with p;
+      assert ((io_pre h ORead args /\ (forall (lt':local_trace h) (r':io_res ORead args). (io_post h ORead args r' /\ lt' == [op_to_ev ORead args r']) ==> theta (io_bind #t1 #t2 (cont_m r') k) (h++lt') (fun lt'' r'' -> p (lt' @ lt'') r''))) ==> p ([EvRead args res]@tl) fs_r);
+      assert (io_pre h ORead args);
+      introduce forall (lt':local_trace h) (r':io_res ORead args). (lt' == [op_to_ev ORead args r']) ==> theta (io_bind #t1 #t2 (cont_m r') k) (h++lt') (fun lt'' r'' -> p (lt' @ lt'') r'') with begin
+        introduce _ ==> _ with _. begin
+          assume (theta (io_bind #t1 #t2 (cont_m r') k) (h++lt') (fun lt'' r'' -> p (lt' @ lt'') r''))
+          //admit ()
+        end
+      end
+    end
+  end
+
+let destruct_fs_beh_ #t1 #t2 (m:io t1) (k:t1 -> io t2) (h:history) (lt:local_trace h) (fs_r:t2) :
+  Lemma (requires thetaP (io_bind m k) h lt fs_r)
+        (ensures exists (lt1:local_trace h) (lt2:local_trace (h++lt1)) (fs_m:t1).
+          lt == (lt1@lt2) /\
+          thetaP m h lt1 fs_m /\
+          thetaP (k fs_m) (h++lt1) lt2 fs_r)
+        (decreases m) =
+  let p : hist_post h t2 = fun (lt:local_trace h) (fs_r:t2) -> exists (lt1:local_trace h) (lt2:local_trace (h++lt1)) (fs_m:t1). lt == (lt1@lt2) /\ thetaP m h lt1 fs_m /\ thetaP (k fs_m) (h++lt1) lt2 fs_r in
+  assert (forall (p:hist_post h t2). theta (io_bind m k) h p ==> p lt fs_r);
+  theta_monad_morphism_bind m k;
+  eliminate forall (p:hist_post h t2). theta m h (fun (lt':local_trace h) (r:t1) -> theta (k r) (h++lt') (fun (lt'':local_trace (h++lt')) (r':t2) -> p (lt' @ lt'') r')) ==> p lt fs_r with p;
+  let _ : hist_post h t1 = (fun (lt':local_trace h) (r:t1) -> theta (k r) (h++lt') (fun (lt'':local_trace (h++lt')) (r':t2) -> exists (lt1:local_trace h) (lt2:local_trace (h++lt1)) (fs_m:t1). (lt'@lt'') == (lt1@lt2) /\ thetaP m h lt1 fs_m /\ thetaP (k fs_m) (h++lt1) lt2 r')) in
+  let p' = hist_post_bind (fun (lt':local_trace h) (r:t1) -> theta (k r) (h++lt') (fun (lt'':local_trace (h++lt')) (r':t2) -> exists (lt1:local_trace h) (lt2:local_trace (h++lt1)) (fs_m:t1). (lt'@lt'') == (lt1@lt2) /\ thetaP m h lt1 fs_m /\ thetaP (k fs_m) (h++lt1) lt2 r')) (fun (lt':local_trace h) (r:t1) -> (fun (lt'':local_trace (h++lt')) (r':t2) -> exists (lt1:local_trace h) (lt2:local_trace (h++lt1)) (fs_m:t1). (lt'@lt'') == (lt1@lt2) /\ thetaP m h lt1 fs_m /\ thetaP (k fs_m) (h++lt1) lt2 r')) in
+  assert (p' == (fun (lt:local_trace h) (b:t2) -> exists (a:t1) (lta:local_trace h) (ltb:local_trace (h++lta)). theta (k a) (h++lta) (fun (lt'':local_trace (h++lta)) (r':t2) -> exists (lt1:local_trace h) (lt2:local_trace (h++lt1)) (fs_m:t1). (lta@lt'') == (lt1@lt2) /\ thetaP m h lt1 fs_m /\ thetaP (k fs_m) (h++lt1) lt2 r') /\ lta@ltb == lt /\ exists (lt1:local_trace h) (lt2:local_trace (h++lt1)) (fs_m:t1). (lta@ltb) == (lt1@lt2) /\ thetaP m h lt1 fs_m /\ thetaP (k fs_m) (h++lt1) lt2 b)) by (FStar.Tactics.compute ());
+  admit ()
+  //assume (theta m h (fun (lt':local_trace h) (r:t1) -> theta (k r) (h++lt') (fun (lt'':local_trace (h++lt')) (r':t2) -> exists (lt1:local_trace h) (lt2:local_trace (h++lt1)) (fs_m:t1). (lt'@lt'') == (lt1@lt2) /\ thetaP m h lt1 fs_m /\ thetaP (k fs_m) (h++lt1) lt2 r')))
+  //admit ()
+  //assume (theta m h (fun (lt':local_trace h) (r:t1) -> theta (k r) (h++lt') (fun (lt'':local_trace (h++lt')) (r':t2) -> p (lt' @ lt'') r')))
+  //admit ()
+  (*assert (forall p. theta (io_bind m k) h p ==> p lt fs_r);
+  theta_monad_morphism_bind m k;
+  assert (forall p. theta m h (fun (lt':local_trace h) (r:t1) -> theta (k r) (h++lt') (fun (lt'':local_trace (h++lt')) (r':t2) -> p (lt' @ lt'') r')) ==> p lt fs_r);
+  more_testing' m k h lt fs_r;
+  assert (forall (p:hist_post h t2). theta (io_bind m k) h (hist_post_bind (fun (lt':local_trace h) (r:t1) -> theta (k r) (h++lt') (fun (lt'':local_trace (h++lt')) (r':t2) -> p (lt' @ lt'') r')) (fun (lt:local_trace h) (r:t1) -> (fun (lt':local_trace (h++lt)) (r':t2) -> r' == fs_r))) ==> (hist_post_bind (fun (lt':local_trace h) (r:t1) -> theta (k r) (h++lt') (fun (lt'':local_trace (h++lt')) (r':t2) -> p (lt' @ lt'') r')) (fun (lt:local_trace h) (r:t1) -> (fun (lt':local_trace (h++lt)) (r':t2) -> r' == fs_r))) lt fs_r);*)
+  
+  //assert (forall p. theta (io_bind m k) h (hist_post_bind (fun (lt':local_trace h) (r:t1) -> theta (k r) (h++lt') (fun (lt'':local_trace (h++lt')) (r':t2) -> p (lt' @ lt'') r')) (fun (lt:local_trace h) (r:t1) -> (fun (lt':local_trace (h++lt)) (r':t2) -> r' == fs_r))) ==> p lt fs_r);
+  //admit ()
+    
+
+  (*match m with
+  | Return x -> admit ()
+  | Call o args func -> begin
+    match o with
+    | ORead -> begin
+    assert (thetaP (io_bind (Call o args func) k) h lt fs_r);
+    assert (wp2p (theta (io_bind (Call o args func) k)) h lt fs_r);
+    assert (wp2p (theta (Call o args (fun i -> io_bind #t1 #t2 (func i) k))) h lt fs_r);
+    assert (forall p. (theta (io_bind m k)) h p ==> p lt fs_r);
+    assert (forall (p:hist_post h t2). (theta (Call o args (fun (i:io_res o args) -> io_bind #t1 #t2 (func i) k))) h p ==> p lt fs_r);
+    assert (forall p. hist_bind (op_wp o args) (fun r -> theta ((fun i -> io_bind #t1 #t2 (func i) k) r)) h p ==> p lt fs_r);
+    assert (forall p. hist_bind (op_wp o args) (fun r -> theta (io_bind #t1 #t2 (func r) k)) h p ==> p lt fs_r);
+    assert (forall p. (op_wp o args) h (hist_post_bind' (fun r -> theta (io_bind #t1 #t2 (func r) k)) p) ==> p lt fs_r);
+    assert (forall p. (to_hist (fun h -> io_pre h o args) (fun h res lt -> io_post h o args res /\ lt == [op_to_ev o args res])) h (hist_post_bind' (fun r -> theta (io_bind #t1 #t2 (func r) k)) p) ==> p lt fs_r);
+    assert (forall p. (to_hist (fun h -> io_pre h o args) (fun h res lt -> io_post h o args res /\ lt == [op_to_ev o args res])) h (hist_post_bind' (fun r -> theta (io_bind #t1 #t2 (func r) k)) p) <==> (io_pre h o args /\ (forall (lt':local_trace h) (r':io_res o args). (io_post h o args r' /\ lt' == [op_to_ev o args r']) ==> theta (io_bind #t1 #t2 (func r') k) (h++lt') (fun lt'' r'' -> p (lt' @ lt'') r''))));
+    assert (forall (p:hist_post h t2). (io_pre h o args /\ (forall (lt':local_trace h) (r':io_res o args). (io_post h o args r' /\ lt' == [op_to_ev o args r']) ==> theta (io_bind #t1 #t2 (func r') k) (h++lt') (fun (lt'':local_trace (h++lt')) (r'':t2) -> p (lt' @ lt'') r''))) ==> p lt fs_r);
+    match lt with
+    | [] -> begin
+    assert (forall (p:hist_post h t2). (forall (lt':local_trace h) (r':io_res o args). (io_post h o args r' /\ lt' == [op_to_ev o args r']) ==> theta (io_bind #t1 #t2 (func r') k) (h++lt') (fun (lt'':local_trace (h++lt')) (r'':t2) -> p (lt' @ lt'') r'')) ==> p lt fs_r);
+    let p : hist_post h t2 = fun (lt_:local_trace h) (fs_r_:t2) -> exists (lt':local_trace h) (lt'':local_trace (h++lt')) (r'':t2). (lt_ == (lt' @ lt'')) /\ (fs_r_ == r'') in
+    assert (forall (r':io_res o args). (io_post h o args r' /\ [] == [op_to_ev o args r']) ==> theta (io_bind #t1 #t2 (func r') k) (h++[]) (fun (lt'':local_trace (h++[])) (r'':t2) -> p ([] @ lt'') r'') ==> p lt fs_r);
+    admit ()
+    end
+    | ev::tl -> begin
+    assert (forall (p:hist_post h t2). (forall (lt':local_trace h) (r':io_res o args). (io_post h o args r' /\ lt' == [op_to_ev o args r']) ==> theta (io_bind #t1 #t2 (func r') k) (h++lt') (fun (lt'':local_trace (h++lt')) (r'':t2) -> p (lt' @ lt'') r'')) ==> p lt fs_r);
+    let p : hist_post h t2 = fun (lt_:local_trace h) (fs_r_:t2) -> exists (lt':local_trace h) (lt'':local_trace (h++lt')) (r'':t2). (lt_ == (lt' @ lt'')) /\ (fs_r_ == r'') in
+    assert (theta (io_bind m k) h p ==> p lt fs_r);
+    assume ((forall (lt':local_trace h) (r':io_res o args). (io_post h o args r' /\ lt' == [op_to_ev o args r']) ==> theta (io_bind #t1 #t2 (func r') k) (h++lt') (fun (lt'':local_trace (h++lt')) (r'':t2) -> p (lt' @ lt'') r'')) ==> p lt fs_r); //by (FStar.Tactics.compute ());
+    introduce forall (lt':local_trace h) (r':io_res o args). (io_post h o args r' /\ lt' == [op_to_ev o args r']) ==> theta (io_bind #t1 #t2 (func r') k) (h++lt') (fun (lt'':local_trace (h++lt')) (r'':t2) -> p (lt' @ lt'') r'') with begin
+      introduce _ ==> _ with _. begin
+        assume (theta (io_bind #t1 #t2 (func r') k) (h++lt') (fun (lt'':local_trace (h++lt')) (r'':t2) -> p (lt' @ lt'') r''))
+      end
+    end;
+    assert (p lt fs_r);
+    let (| op_, a_, r_ |) = destruct_ev ev in
+    
+    admit ()
+    end
+    end
+    | _ -> admit ()
+    end
+
+
+    theta_monad_morphism_bind m k;
+    assert (forall (p:hist_post h t2). theta m h (fun (lt':local_trace h) (r':t1) -> theta (k r') (h++lt') (fun (lt'':local_trace (h++lt')) (r'':t2) -> p (lt' @ lt'') r'')) ==> p lt fs_r);
+
+
+(*let theta_lemma #a #b (args:io_args ORead) (res:io_res ORead args) (func:io_res ORead args -> io a) (k:a -> io b) (h:history) (tl:local_trace ((EvRead args res)::h)) (fs_r:b) :
+  Lemma 
+    (requires wp2p (theta (io_bind (Call ORead args func) k)) h ([EvRead args res]@tl) fs_r)
+    (ensures wp2p (theta (k *)
+
+let destruct_fs_beh_read #t1 #t2 (args:io_args ORead) (res:io_res ORead args) (cont_m:io_res ORead args -> io t1) (k:t1 -> io t2) (h:history) (tl:local_trace ((EvRead args res)::h)) (fs_r:t2) :
+  Lemma (requires exists (p:hist_post h t2). theta (io_bind (Call ORead args cont_m) k) h p ==> p ([EvRead args res]@tl) fs_r)
+        (ensures exists (p':hist_post ((EvRead args res)::h) t2). theta (io_bind (cont_m res) k) ((EvRead args res)::h) p' ==> p' tl fs_r) =
+  eliminate exists (p:hist_post h t2). theta (io_bind (Call ORead args cont_m) k) h p ==> p ([EvRead args res]@tl) fs_r
+  returns exists (p':hist_post ((EvRead args res)::h) t2). theta (io_bind (cont_m res) k) ((EvRead args res)::h) p' ==> p' tl fs_r with _. begin
+    let p' : hist_post ((EvRead args res)::h) t2 = (fun (lt'':local_trace ((EvRead args res)::h)) (r'':t2) -> p ([EvRead args res]@lt'') r'') in
+    assert (theta (io_bind (Call ORead args cont_m) k) h p ==> p ([EvRead args res]@tl) fs_r);
+    assert (theta (Call ORead args (fun (i:io_res ORead args) -> io_bind #t1 #t2 (cont_m i) k)) h p ==> p ([EvRead args res]@tl) fs_r);
+    assert (hist_bind (op_wp ORead args) (fun r -> theta ((fun i -> io_bind #t1 #t2 (cont_m i) k) r)) h p ==> p ([EvRead args res]@tl) fs_r);
+    assert (hist_bind (op_wp ORead args) (fun r -> theta (io_bind #t1 #t2 (cont_m r) k)) h p ==> p ([EvRead args res]@tl) fs_r);
+    assert ((op_wp ORead args) h (hist_post_bind' (fun r -> theta (io_bind #t1 #t2 (cont_m r) k)) p) ==> p ([EvRead args res]@tl) fs_r);
+    assert ((to_hist (fun h -> io_pre h ORead args) (fun h res lt -> io_post h ORead args res /\ lt == [op_to_ev ORead args res])) h (hist_post_bind' (fun r -> theta (io_bind #t1 #t2 (cont_m r) k)) p) ==> p ([EvRead args res]@tl) fs_r);
+    assert ((to_hist (fun h -> io_pre h ORead args) (fun h res lt -> io_post h ORead args res /\ lt == [op_to_ev ORead args res])) h (hist_post_bind' (fun r -> theta (io_bind #t1 #t2 (cont_m r) k)) p) <==> (io_pre h ORead args /\ (forall (lt':local_trace h) (r':io_res ORead args). (io_post h ORead args r' /\ lt' == [op_to_ev ORead args r']) ==> theta (io_bind #t1 #t2 (cont_m r') k) (h++lt') (fun lt'' r'' -> p (lt' @ lt'') r''))));
+      assert ((io_pre h ORead args /\ (forall (lt':local_trace h) (r':io_res ORead args). (io_post h ORead args r' /\ lt' == [op_to_ev ORead args r']) ==> theta (io_bind #t1 #t2 (cont_m r') k) (h++lt') (fun lt'' r'' -> p (lt' @ lt'') r''))) ==> p ([EvRead args res]@tl) fs_r);
+    assert (p' tl fs_r == p ([EvRead args res]@tl) fs_r);
+    introduce theta (io_bind (cont_m res) k) ((EvRead args res)::h) p' ==> p' tl fs_r with _. begin
+      introduce forall (lt':local_trace h) (r':io_res ORead args). (io_post h ORead args r' /\ lt' == [op_to_ev ORead args r']) ==> theta (io_bind #t1 #t2 (cont_m r') k) (h++lt') (fun lt'' r'' -> p (lt' @ lt'') r'') with begin
+        introduce _ ==> _ with _. begin
+          admit ()
+        end
+      end
+    end
+  end
+*)
+
+let destruct_fs_beh #t1 #t2 (m:io t1) (k:t1 -> io t2) (h:history) (lt:local_trace h) (fs_r:t2) :
+  Lemma
+    (requires thetaP (io_bind m k) h lt fs_r) // forall p. theta (io_bind m k) h p ==> p lt fs_r
+    (ensures exists (lt1:local_trace h) (lt2:local_trace (h++lt1)) (fs_m:t1).
+      lt == (lt1@lt2) /\
+      thetaP m h lt1 fs_m /\ // forall p. theta m h p ==> p lt1 fs_m
+      thetaP (k fs_m) (h++lt1) lt2 fs_r) (* forall p. theta (k fs_m) (h++lt1) p ==> p lt2 fs_r *) = 
+    assert (forall (p:hist_post h t2). theta (io_bind m k) h p ==> p lt fs_r);
+    let p : hist_post h t2 = fun (lt:local_trace h) (r:t2) -> exists (lt1:local_trace h) (lt2:local_trace (h++lt1)) (fs_m:t1). (lt==lt1@lt2) /\ thetaP m h lt1 fs_m /\ thetaP (k fs_m) (h++lt1) lt2 fs_r in
+    eliminate forall (p:hist_post h t2). theta (io_bind m k) h p ==> p lt fs_r with p;
+    //assume (theta (io_bind m k) h p)
+    theta_monad_morphism_bind m k;
+    assert (theta (io_bind m k) `hist_equiv` hist_bind (theta m) (fun x -> theta (k x)));
+    eliminate forall (h:history) (p:hist_post h t2). theta (io_bind m k) h p <==> hist_bind (theta m) (fun x -> theta (k x)) h p with h p;
+    assert (hist_bind (theta m) (fun x -> theta (k x)) h p == (theta m) h (hist_post_bind' (fun x -> theta (k x)) p));
+    assert ((theta m) h (hist_post_bind' (fun x -> theta (k x)) p) == (theta m) h (fun lt r -> theta (k r) (h++lt) (hist_post_shift h p lt)));
+    assert ((theta m) h (fun lt r -> theta (k r) (h++lt) (hist_post_shift h p lt)) == (theta m) h (fun lt r -> theta (k r) (h++lt) (fun lt' r' -> p (lt @ lt') r')));
+    //assume ((theta m) h (fun lt r -> theta (k r) (h++lt) (fun lt' r' -> p (lt @ lt') r')))
+    admit ()
+
+
+(* Thoughts with Danel 
+
+forall p. theta (io_bind m k) h p ==> p lt fs_r
+forall q. theta m h q ==> q lt1 fs_m
+
+Instantiate p with: exists lt'. lt == (lt1@lt') /\ q lt1 fs_m
+Prove: theta (io_bind m k) h p
+
+However:
+1. we don't know the values lt1 and fs_m ahead of time
+2. still need to prove: theta (io_bind m k) h p 
+*)
